backends/lean/Base/Diverge/ElabBase.lean
@@ -1,8 +1,11 @@
 import Lean
+import Base.Utils
+import Base.Primitives.Base
 
 namespace Diverge
 
 open Lean Elab Term Meta
+open Utils
 
 -- We can't define and use trace classes in the same file
 initialize registerTraceClass `Diverge.elab
@@ -11,5 +14,8 @@ initialize registerTraceClass `Diverge.def.sigmas
 initialize registerTraceClass `Diverge.def.genBody
 initialize registerTraceClass `Diverge.def.valid
 initialize registerTraceClass `Diverge.def.unfold
+
+-- For the attribute (for higher-order functions)
+initialize registerTraceClass `Diverge.attr
 
 end Diverge
